code/nist-pcurves/Hacl.Impl.PCurves.Field.P384.fst
@@ -1,0 +1,58 @@
+module Hacl.Impl.PCurves.Field.P384
+
+open FStar.Mul
+open FStar.HyperStack.All
+open FStar.HyperStack
+module ST = FStar.HyperStack.ST
+
+open Lib.IntTypes
+open Lib.Buffer
+
+
+module S = Spec.PCurves
+module SM = Hacl.Spec.PCurves.Montgomery
+module CC = Hacl.Impl.PCurves.Constants
+
+open Spec.P384
+open Hacl.Impl.PCurves.Constants.P384
+open Hacl.Impl.PCurves.Bignum.P384
+open Hacl.Impl.PCurves.Field
+
+[@CInline]
+val bn_is_lt_prime_mask: bn_is_lt_prime_mask_t
+let bn_is_lt_prime_mask f = bn_is_lt_prime_mask_g f
+
+[@CInline]
+val fadd: fadd_t
+let fadd a b c = fadd_g a b c
+
+[@CInline]
+val fsub: fsub_t
+let fsub a b c = fsub_g a b c
+
+[@CInline]
+val fmul: fmul_t
+let fmul a b c = fmul_g a b c
+
+[@CInline]
+val fsqr: fsqr_t
+let fsqr a b = fsqr_g a b
+
+[@CInline]
+val from_mont: from_mont_t
+let from_mont a b = from_mont_g a b
+
+[@CInline]
+val to_mont: to_mont_t
+let to_mont a b = to_mont_g a b
+
+inline_for_extraction
+instance p384_field_ops: field_ops = {
+  bn_is_lt_prime_mask;
+  fadd;
+  fsub;
+  fmul;
+  fsqr;
+  from_mont;
+  to_mont
+}
