code/nist-pcurves/Hacl.Impl.PCurves.Qinv.P384.fst
@@ -1,0 +1,104 @@
+module Hacl.Impl.PCurves.Qinv.P384
+
+open FStar.Mul
+open FStar.HyperStack.All
+open FStar.HyperStack
+module ST = FStar.HyperStack.ST
+
+open Lib.IntTypes
+open Lib.Buffer
+
+module SE = Spec.Exponentiation
+module LE = Lib.Exponentiation
+module BE = Hacl.Impl.Exponentiation
+module BD = Hacl.Spec.Bignum.Definitions
+module LSeq = Lib.Sequence
+module M = Lib.NatMod
+
+module S = Spec.PCurves
+module SI = Hacl.Spec.PCurves.Qinv
+module SI256 = Hacl.Spec.PCurves.Qinv.P384
+module QI = Hacl.Impl.PCurves.Qinv
+module SM = Hacl.Spec.PCurves.Montgomery
+
+open Spec.P384
+open Hacl.Impl.PCurves.Bignum
+open Hacl.Impl.PCurves.Bignum.P384
+open Hacl.Impl.PCurves.Constants
+open Hacl.Impl.PCurves.Constants.P384
+open Hacl.Impl.PCurves.Field
+open Hacl.Impl.PCurves.Field.P384
+open Hacl.Impl.PCurves.Scalar
+open Hacl.Impl.PCurves.Scalar.P384
+open Hacl.Impl.PCurves.InvSqrt
+open Hacl.Impl.PCurves.Qinv
+
+#set-options "--z3rlimit 50 --fuel 0 --ifuel 0"
+
+val qexp_vartime (out a b:felem) : Stack unit
+  (requires fun h ->
+    live h out /\ live h a /\ live h b /\
+    disjoint out a /\ disjoint out b /\
+    as_nat h a < S.order)
+  (ensures  fun h0 _ h1 -> modifies (loc out) h0 h1 /\
+    as_nat h1 out == M.pow_mod #S.order (as_nat h0 a) (as_nat h0 b))
+
+[@CInline]
+let qexp_vartime out a b =
+  let h0 = ST.get () in
+  assert_norm(pow2 5 == 32);
+  bn_v_is_as_nat6 (as_seq h0 b);
+  assume(as_nat h0 b < pow2 384);
+  BE.lexp_fw_vartime 6ul 0ul
+    mk_pcurve_order_concrete_ops 5ul (null uint64) a 6ul 384ul b out;
+  let h1 = ST.get () in
+  SE.exp_fw_lemma SI.mk_nat_mod_concrete_ops (as_nat h0 a) 384 (as_nat h0 b) 5;
+  LE.exp_fw_lemma SI.nat_mod_comm_monoid (as_nat h0 a) 384 (as_nat h0 b) 5;
+  admit();
+  assert (as_nat h1 out == LE.pow SI.nat_mod_comm_monoid (as_nat h0 a) (as_nat h0 b));
+  M.lemma_pow_nat_mod_is_pow #S.order (as_nat h0 a) (as_nat h0 b);
+  assert (as_nat h1 out == M.pow (as_nat h0 a) (as_nat h0 b) % S.order);
+  M.lemma_pow_mod #S.order (as_nat h0 a) (as_nat h0 b)
+
+
+inline_for_extraction noextract
+val make_order384_minus_2: b:felem -> Stack unit
+  (requires fun h -> live h b)
+  (ensures  fun h0 _ h1 -> modifies (loc b) h0 h1 /\
+    as_nat h1 b == S.order - 2)
+
+let make_order384_minus_2 n =
+    // 0xffffffffffffffffffffffffffffffffffffffffffffffffc7634d81f4372ddf581a0db248b0a77aecec196accc52971
+    [@inline_let] let n0 = u64 0xecec196accc52971 in
+    [@inline_let] let n1 = u64 0x581a0db248b0a77a in
+    [@inline_let] let n2 = u64 0xc7634d81f4372ddf in
+    [@inline_let] let n3 = u64 0xffffffffffffffff in
+    [@inline_let] let n4 = u64 0xffffffffffffffff in
+    [@inline_let] let n5 = u64 0xffffffffffffffff in
+    assert_norm (v n0 + v n1 * pow2 64 + v n2 * pow2 128 + v n3 * pow2 192 + v n3 * pow2 256 + v n3 * pow2 320 = Spec.P384.p384_order - 2);
+    bn_make_u64_6 n n0 n1 n2 n3 n4 n5
+
+[@CInline]
+val p384_qinv: res:felem -> a:felem -> Stack unit
+   (requires fun h ->
+     live h a /\ live h res /\ eq_or_disjoint a res /\
+     as_nat h a < S.order)
+   (ensures fun h0 _ h1 -> modifies (loc res) h0 h1 /\
+     as_nat h1 res < S.order /\
+     qmont_as_nat h1 res == S.qinv (qmont_as_nat h0 a))
+
+[@CInline]
+let p384_qinv res a =
+  push_frame ();
+  let b = create 6ul (u64 0) in
+  make_order384_minus_2 b;
+  qexp_vartime res a b;
+  admit();
+  pop_frame ()
+
+inline_for_extraction
+instance p384_inv_sqrt : curve_inv_sqrt = {
+  finv = Hacl.Impl.PCurves.Finv.P384.p384_finv;
+  qinv = p384_qinv;
+  fsqrt = Hacl.Impl.PCurves.Finv.P384.p384_fsqrt
+}
