code/nist-pcurves/Hacl.P384.fst
@@ -1,4 +1,4 @@
-module Hacl.P256
+module Hacl.P384
 
 open FStar.Mul
 open FStar.HyperStack.All
@@ -21,15 +21,16 @@ module S = Spec.PCurves
 module BN = Hacl.Impl.PCurves.Bignum
 module P = Hacl.Impl.PCurves.Point
 
-open Hacl.Impl.PCurves.Bignum.P256
-open Hacl.Impl.PCurves.Constants.P256
-open Hacl.Impl.PCurves.Field.P256
-open Hacl.Impl.PCurves.Scalar.P256
-open Hacl.Impl.PCurves.Finv.P256
-open Hacl.Impl.PCurves.Qinv.P256
-open Hacl.Impl.PCurves.Group.P256
-open Hacl.Impl.PCurves.PrecompTable.P256
-open Hacl.Impl.PCurves.PointMul.P256
+open Spec.P384
+open Hacl.Impl.PCurves.Bignum.P384
+open Hacl.Impl.PCurves.Constants.P384
+open Hacl.Impl.PCurves.Field.P384
+open Hacl.Impl.PCurves.Scalar.P384
+open Hacl.Impl.PCurves.Finv.P384
+open Hacl.Impl.PCurves.Qinv.P384
+open Hacl.Impl.PCurves.Group.P384
+open Hacl.Impl.PCurves.PrecompTable.P384
+open Hacl.Impl.PCurves.PointMul.P384
 
 #set-options "--z3rlimit 30 --fuel 0 --ifuel 0"
 
@@ -52,31 +53,31 @@ let msg_as_felem alg msg_len msg res =
 
   [@inline_let] let sz: size_t =
     match alg with
-    | S.NoHash -> 32ul
+    | S.NoHash -> 48ul
     | S.Hash a -> Hacl.Hash.Definitions.hash_len a in
 
   let mHash = create sz (u8 0) in
 
   begin
   match alg with
-    | S.NoHash -> copy mHash (sub msg 0ul 32ul)
+    | S.NoHash -> copy mHash (sub msg 0ul 48ul)
     | S.Hash a -> match a with
       | SHA2_256 -> Hacl.Streaming.SHA2.hash_256 msg msg_len mHash
       | SHA2_384 -> Hacl.Streaming.SHA2.hash_384 msg msg_len mHash
       | SHA2_512 -> Hacl.Streaming.SHA2.hash_512 msg msg_len mHash
   end;
   LowStar.Ignore.ignore msg_len;
-  let mHash32 = sub mHash 0ul 32ul in
-  BN.bn_from_bytes_be res mHash32;
+  let mHash48 = sub mHash 0ul 48ul in
+  BN.bn_from_bytes_be res mHash48;
   qmod_short res res;
   pop_frame ()
 
 [@ CInline ]
 val ecdsa_sign_msg_as_qelem:
-    signature:lbuffer uint8 (2ul *. 32ul)
+    signature:lbuffer uint8 (2ul *. 48ul)
   -> m_q:BN.felem
-  -> private_key:lbuffer uint8 32ul
-  -> nonce:lbuffer uint8 32ul ->
+  -> private_key:lbuffer uint8 48ul
+  -> nonce:lbuffer uint8 48ul ->
   Stack bool
   (requires fun h ->
     live h signature /\ live h m_q /\ live h private_key /\ live h nonce /\
@@ -90,23 +91,23 @@ val ecdsa_sign_msg_as_qelem:
 
 let ecdsa_sign_msg_as_qelem signature m_q private_key nonce =
   ecdsa_sign_msg_as_qelem
-  #p256_params
-  #p256_bn_ops
-  #p256_curve_constants
-  #p256_field_ops
-  #p256_order_ops
-  #p256_inv_sqrt
-  #p256_point_ops
-  #p256_precomp_tables
-  #p256_point_mul_ops
+  #p384_params
+  #p384_bn_ops
+  #p384_curve_constants
+  #p384_field_ops
+  #p384_order_ops
+  #p384_inv_sqrt
+  #p384_point_ops
+  #p384_precomp_tables
+  #p384_point_mul_ops
   signature m_q private_key nonce
  
 [@ CInline ]
 val ecdsa_verify_msg_as_qelem:
     m_q:BN.felem
-  -> public_key:lbuffer uint8 (2ul *. 32ul)
-  -> signature_r:lbuffer uint8 32ul
-  -> signature_s:lbuffer uint8 32ul ->
+  -> public_key:lbuffer uint8 (2ul *. 48ul)
+  -> signature_r:lbuffer uint8 48ul
+  -> signature_s:lbuffer uint8 48ul ->
   Stack bool
   (requires fun h ->
     live h public_key /\ live h signature_r /\ live h signature_s /\ live h m_q /\
@@ -117,22 +118,22 @@ val ecdsa_verify_msg_as_qelem:
 
 let ecdsa_verify_msg_as_qelem m_q public_key signature_r signature_s =
   ecdsa_verify_msg_as_qelem
-  #p256_params
-  #p256_bn_ops
-  #p256_curve_constants
-  #p256_field_ops
-  #p256_order_ops
-  #p256_inv_sqrt
-  #p256_point_ops
-  #p256_precomp_tables
-  #p256_point_mul_ops
+  #p384_params
+  #p384_bn_ops
+  #p384_curve_constants
+  #p384_field_ops
+  #p384_order_ops
+  #p384_inv_sqrt
+  #p384_point_ops
+  #p384_precomp_tables
+  #p384_point_mul_ops
   m_q public_key signature_r signature_s
 
 inline_for_extraction noextract
-val ecdsa_signature: alg:S.hash_alg_ecdsa -> ecdsa_sign_p256_st alg
+val ecdsa_signature: alg:S.hash_alg_ecdsa -> ecdsa_sign_p384_st alg
 let ecdsa_signature alg signature msg_len msg private_key nonce =
   push_frame ();
-  let m_q = BN.create_felem #p256_params in
+  let m_q = BN.create_felem #p384_params in
   msg_as_felem alg msg_len msg m_q;
   let res = ecdsa_sign_msg_as_qelem signature m_q private_key nonce in
   pop_frame ();
@@ -140,36 +141,36 @@ let ecdsa_signature alg signature msg_len msg private_key nonce =
 
 
 inline_for_extraction noextract
-val ecdsa_verification: alg:S.hash_alg_ecdsa -> ecdsa_verify_p256_st alg
+val ecdsa_verification: alg:S.hash_alg_ecdsa -> ecdsa_verify_p384_st alg
 let ecdsa_verification alg msg_len msg public_key signature_r signature_s =
   push_frame ();
-  let m_q = BN.create_felem #p256_params in
+  let m_q = BN.create_felem #p384_params in
   msg_as_felem alg msg_len msg m_q;
   let res = ecdsa_verify_msg_as_qelem m_q public_key signature_r signature_s in
   pop_frame ();
   res
 
 
-let ecdsa_sign_p256_sha2 signature msg_len msg private_key nonce =
+let ecdsa_sign_p384_sha2 signature msg_len msg private_key nonce =
   ecdsa_signature (S.Hash SHA2_256) signature msg_len msg private_key nonce
 
-let ecdsa_sign_p256_sha384 signature msg_len msg private_key nonce =
+let ecdsa_sign_p384_sha384 signature msg_len msg private_key nonce =
   ecdsa_signature (S.Hash SHA2_384) signature msg_len msg private_key nonce
 
-let ecdsa_sign_p256_sha512 signature msg_len msg private_key nonce =
+let ecdsa_sign_p384_sha512 signature msg_len msg private_key nonce =
   ecdsa_signature (S.Hash SHA2_512) signature msg_len msg private_key nonce
 
-let ecdsa_sign_p256_without_hash signature msg_len msg private_key nonce =
+let ecdsa_sign_p384_without_hash signature msg_len msg private_key nonce =
   ecdsa_signature S.NoHash signature msg_len msg private_key nonce
 
 
-let ecdsa_verif_p256_sha2 msg_len msg public_key signature_r signature_s =
+let ecdsa_verif_p384_sha2 msg_len msg public_key signature_r signature_s =
   ecdsa_verification (S.Hash SHA2_256) msg_len msg public_key signature_r signature_s
 
-let ecdsa_verif_p256_sha384 msg_len msg public_key signature_r signature_s =
+let ecdsa_verif_p384_sha384 msg_len msg public_key signature_r signature_s =
   ecdsa_verification (S.Hash SHA2_384) msg_len msg public_key signature_r signature_s
 
-let ecdsa_verif_p256_sha512 msg_len msg public_key signature_r signature_s =
+let ecdsa_verif_p384_sha512 msg_len msg public_key signature_r signature_s =
   ecdsa_verification (S.Hash SHA2_512) msg_len msg public_key signature_r signature_s
 
 let ecdsa_verif_without_hash msg_len msg public_key signature_r signature_s =
@@ -178,7 +179,7 @@ let ecdsa_verif_without_hash msg_len msg public_key signature_r signature_s =
 
 let validate_public_key public_key =
   push_frame ();
-  let point_jac = P.create_point #p256_params in
+  let point_jac = P.create_point #p384_params in
   let res = P.load_point_vartime point_jac public_key in
   pop_frame ();
   res
@@ -186,7 +187,7 @@ let validate_public_key public_key =
 
 let validate_private_key private_key =
   push_frame ();
-  let bn_sk = BN.create_felem #p256_params in
+  let bn_sk = BN.create_felem #p384_params in
   BN.bn_from_bytes_be bn_sk private_key;
   let res = Hacl.Impl.PCurves.Scalar.bn_is_lt_order_and_gt_zero_mask bn_sk in
   pop_frame ();
@@ -208,26 +209,26 @@ let raw_to_compressed pk_raw pk =
 
 let dh_initiator public_key private_key =
   Hacl.Impl.PCurves.DH.ecdh_i
-  #p256_params
-  #p256_bn_ops
-  #p256_curve_constants
-  #p256_field_ops
-  #p256_order_ops
-  #p256_inv_sqrt
-  #p256_point_ops
-  #p256_precomp_tables
-  #p256_point_mul_ops
+  #p384_params
+  #p384_bn_ops
+  #p384_curve_constants
+  #p384_field_ops
+  #p384_order_ops
+  #p384_inv_sqrt
+  #p384_point_ops
+  #p384_precomp_tables
+  #p384_point_mul_ops
   public_key private_key
 
 let dh_responder shared_secret their_pubkey private_key =
   Hacl.Impl.PCurves.DH.ecdh_r
-  #p256_params
-  #p256_bn_ops
-  #p256_curve_constants
-  #p256_field_ops
-  #p256_order_ops
-  #p256_inv_sqrt
-  #p256_point_ops
-  #p256_precomp_tables
-  #p256_point_mul_ops
+  #p384_params
+  #p384_bn_ops
+  #p384_curve_constants
+  #p384_field_ops
+  #p384_order_ops
+  #p384_inv_sqrt
+  #p384_point_ops
+  #p384_precomp_tables
+  #p384_point_mul_ops
   shared_secret their_pubkey private_key
