specs/Spec.P384.fst
@@ -1,0 +1,78 @@
+module Spec.P384
+open FStar.Mul
+open Lib.IntTypes
+open Lib.Sequence
+open Lib.ByteSequence
+
+open Spec.PCurves
+
+///  P-384 Curve Parameters
+
+inline_for_extraction noextract
+let p384_bits = 384
+
+inline_for_extraction noextract
+let p384_bytes : (x:nat{8 * x >= p384_bits}) = 48
+
+
+// Prime  0xfffffffffffffffffffffffffffffffffffffffffffffffffffffffffffffffeffffffff0000000000000000ffffffff
+inline_for_extraction noextract
+let p384_prime: (a:pos{a = 0xfffffffffffffffffffffffffffffffffffffffffffffffffffffffffffffffeffffffff0000000000000000ffffffff /\ a < pow2 384}) =
+  let p = pow2 384 - pow2 128 - pow2 96 + pow2 32 - 1 in
+  assert_norm (0xfffffffffffffffffffffffffffffffffffffffffffffffffffffffffffffffeffffffff0000000000000000ffffffff = p);
+  assert_norm (p < pow2 384); p
+
+inline_for_extraction noextract
+let p384_order: (a:pos{a < pow2 384}) =
+  let o = 0xffffffffffffffffffffffffffffffffffffffffffffffffc7634d81f4372ddf581a0db248b0a77aecec196accc52973 in
+  assert_norm (o < pow2 384); o
+
+inline_for_extraction noextract
+let p384_a_coeff : (x:pos{x < p384_prime}) = (-3) % p384_prime
+let p384_b_coeff : (x:pos{x < p384_prime}) =
+  let b = 0xb3312fa7e23ee7e4988e056be3f82d19181d9c6efe8141120314088f5013875ac656398d8a2ed19d2a85c8edd3ec2aef in
+  assert_norm (b < p384_prime); b
+
+inline_for_extraction noextract
+let p384_basepoint_x : (x:pos{x < p384_prime}) =
+  let x = 0xaa87ca22be8b05378eb1c71ef320ad746e1d3b628ba79b9859f741e082542a385502f25dbf55296c3a545e3872760ab7 in
+  assert_norm (x < p384_prime); x
+
+inline_for_extraction noextract
+let p384_basepoint_y : (x:pos{x < p384_prime}) =
+  let y = 0x3617de4a96262c6f5d9e98bf9292dc29f8f41dbd289a147ce9da3113b5f0b8c00a60b1ce1d7e819d7a431d7c90ea0e5f in
+  assert_norm (y < p384_prime); y
+
+inline_for_extraction noextract
+let p384_mont_mu: (x:uint64{(1 + p384_prime * v x) % pow2 64 == 0}) =
+  assert_norm((1 + p384_prime * 4294967297) % pow2 64 == 0);
+  u64 4294967297
+
+inline_for_extraction noextract
+let p384_mont_q_mu: (x:uint64{(1 + p384_order * v x) % pow2 64 == 0}) =
+  assert_norm((1 + p384_order * 7986114184663260229) % pow2 64 == 0);
+  u64 7986114184663260229
+
+inline_for_extraction noextract
+let p384_bn_limbs: (x:size_t{v x = (p384_bytes + 7) / 8}) =
+  assert_norm(6 == (p384_bytes + 7) / 8);
+  size 6
+
+inline_for_extraction noextract
+instance p384_params : curve_params = {
+  bits = p384_bits;
+  bytes = p384_bytes;
+  size_bytes = 48ul;
+  prime = p384_prime;
+  order = p384_order;
+  basepoint_x = p384_basepoint_x;
+  basepoint_y = p384_basepoint_y;
+  a_coeff = p384_a_coeff;
+  b_coeff = p384_b_coeff;
+  mont_mu = p384_mont_mu;
+  mont_q_mu = p384_mont_q_mu;
+  bn_limbs = p384_bn_limbs
+}
+
+let p384_basepoint : proj_point #p384_params =
+  (p384_basepoint_x,p384_basepoint_y,one)
